changes from last time

HumanProof/Basic.lean
@@ -5,69 +5,68 @@ namespace HumanProof
 open Lean Meta
 
 inductive Box : Type where
-| forallB (name : Name) (type : Expr) (body : Box)
-| metaVar (name : Name) (type : Expr) (body : Box)
+| forallB (decl : LocalDecl) (body : Box) (hidden : Bool := false)
+| metaVar (mvarId : MVarId) (decl : MetavarDecl) (body : Box)
 | result (r : Expr)
-| and (name : Name) (type : Expr) (value body : Box)
+| and (decl : LocalDecl) (value body : Box)
 | or (inl : Box) (inr : Box)
--- | letB (name : Name) (type value : Expr) (body : Box)
+| haveB (decl : LocalDecl) (value : Expr) (body : Box)
 deriving Inhabited
 
 namespace Box
 
-def getResults : Box → Array Expr
-  | .forallB name type body =>
-    (getResults body).map (.forallE name type · .default)
-  | metaVar _ _ body =>
-    (getResults body).filterMap fun e =>
-      if e.hasLooseBVar 0 then
-        none
-      else
-        some (e.lowerLooseBVars 1 1)
-  | .result r => #[r]
-  | .and name type inl inr =>
-    (getResults inl).flatMap fun e =>
-      (getResults inr).map (mkLet name type e ·)
-  | .or inl inr =>
-    getResults inl ++ getResults inr
+-- def getResults : Box → Array Expr
+--   | .forallB name type body =>
+--     (getResults body).map (.forallE name type · .default)
+--   | metaVar _ _ body =>
+--     (getResults body).filterMap fun e =>
+--       if e.hasLooseBVar 0 then
+--         none
+--       else
+--         some (e.lowerLooseBVars 1 1)
+--   | .result r => #[r]
+--   | .and name type inl inr =>
+--     (getResults inl).flatMap fun e =>
+--       (getResults inr).map (mkLet name type e ·)
+--   | .or inl inr =>
+--     getResults inl ++ getResults inr
 
 
 inductive Coord where
-  | forallB | metaVar | andL | andR | orL | orR
+  | forallB | metaVar | andL | andR | orL | orR | haveB
   deriving Repr
 
 inductive PathItem where
-  | forallB (name : Name) (type : Expr)
-  | metaVar (name : Name) (type : Expr)
-  | andL (name : Name) (type : Expr) (body : Box)
-  | andR (name : Name) (type : Expr) (value : Box)
+  | forallB (decl : LocalDecl) (hidden : Bool)
+  | metaVar (mvarId : MVarId) (decl : MetavarDecl)
+  | andL (decl : LocalDecl) (body : Box)
+  | andR (decl : LocalDecl) (value : Box)
   | orL (inr : Box)
   | orR (inl : Box)
+  | haveB (decl : LocalDecl) (value : Expr)
 
 structure Zipper where
   path           : List PathItem
   cursor         : Box
-  vars           : Array Expr
   lctx           : LocalContext
   localInstances : LocalInstances
   mctx           : MetavarContext
 
 def Zipper.up (zipper : Zipper) : Option Zipper := do
   let item :: path := zipper.path | failure
-  let { cursor, vars, .. } := zipper
+  let { cursor, .. } := zipper
   let zipper := { zipper with path }
   match item with
-  | .forallB name type =>
-    let fvar := vars.back!
+  | .forallB decl hidden =>
     return { zipper with
-      cursor := .forallB name type cursor
-      lctx   := zipper.lctx.erase fvar.fvarId!
-      vars   := vars.pop }
-  | .metaVar name type => return { zipper with cursor := .metaVar name type cursor, vars := vars.pop }
-  | .andL name type body => return { zipper with cursor := .and name type cursor body }
-  | .andR name type value => return { zipper with cursor := .and name type value cursor }
+      cursor := .forallB decl cursor hidden
+      lctx   := zipper.lctx.erase decl.fvarId  }
+  | .metaVar mvarId decl => return { zipper with cursor := .metaVar mvarId decl cursor }
+  | .andL decl body => return { zipper with cursor := .and decl cursor body }
+  | .andR decl value => return { zipper with cursor := .and decl value cursor }
   | .orL inr => return { zipper with cursor := .or cursor inr }
   | .orR inl => return { zipper with cursor := .or inl cursor }
+  | .haveB decl value => return { zipper with cursor := .haveB decl value cursor }
 
 partial def Zipper.zip (zipper : Zipper) : Box :=
   if let some zipper := zipper.up then
@@ -76,35 +75,33 @@ partial def Zipper.zip (zipper : Zipper) : Box :=
     zipper.cursor
 
 def Zipper.down (zipper : Zipper) (coord : Coord) : MetaM Zipper := do
-  let { path, cursor, vars, lctx, localInstances, mctx ..} := zipper
-  let withFVar (name : Name) (type : Expr) (pathItem : PathItem) (body : Box) : MetaM Zipper := do
+  let { path, cursor, lctx, localInstances, mctx ..} := zipper
+  let withFVar (decl : LocalDecl) (pathItem : PathItem) (body : Box) : MetaM Zipper := do
     withLCtx lctx localInstances do
-      withLocalDeclD name type fun fvar => do
+      withExistingLocalDecls [decl] do
         return { zipper with
           path := pathItem :: path
           cursor := body
-          vars := vars.push fvar
           lctx := ← getLCtx
           localInstances := ← getLocalInstances }
   match coord, cursor with
-  | .forallB, .forallB name type body => withFVar name type (.forallB name type) body
-  | .metaVar, .metaVar name type body =>
-    setMCtx mctx
-    let mvar ← mkFreshExprMVarAt lctx localInstances type (kind := .syntheticOpaque) (userName := name)
+  | .forallB, .forallB decl body hidden => withFVar decl (.forallB decl hidden) body
+  | .metaVar, .metaVar mvarId decl body =>
+    let {userName, lctx, type, localInstances, kind, .. } := decl
     return { zipper with
-      path := .metaVar name type :: path
+      path := .metaVar mvarId decl :: path
       cursor := body
-      vars := vars.push mvar
-      mctx := ← getMCtx}
-  | .andL   , .and name type value body => return { zipper with path := .andL name type body :: path, cursor := value }
-  | .andR   , .and name type value body => withFVar name type (.andR name type value) body
+      mctx := mctx.addExprMVarDeclExp mvarId userName lctx localInstances type kind }
+  | .andL   , .and decl value body => return { zipper with path := .andL decl body :: path, cursor := value }
+  | .andR   , .and decl value body => withFVar decl (.andR decl value) body
   | .orL    , .or inl inr => return { zipper with path := .orL inr :: path, cursor := inl }
   | .orR    , .or inl inr => return { zipper with path := .orR inl :: path, cursor := inr }
+  | .haveB  , .haveB decl value body => withFVar decl (.haveB decl value) body
   | _       , _ => throwError "Zipper down coordinate is wrong: {repr coord}"
 
 
 def Zipper.unzip (box : Box) (address : List Coord) : MetaM Zipper := do
-  go { path := [], cursor := box, vars := #[], lctx := {}, localInstances := {}, mctx := {} } address
+  go { path := [], cursor := box, lctx := {}, localInstances := {}, mctx := {} } address
 where
   go (zipper : Zipper) (address : List Coord) : MetaM Zipper := do
     let coord :: address := address | return zipper
@@ -113,10 +110,95 @@ where
 
 
 
+example (h : 1 + 1 = 2) (g : False) (hh : h = h) : True := by
+  change 2 = 2 at  h
+  simp at h
+
+/-
+(1) define addMVar and assign mvar.
+  - define/find metavariable dependency relation.
+  -
+(2) DONE -- collectDelayMVarApps : Expr → MetaM (HashSet MVarId × HashMap MvarId (Array Expr))
+
+(3) DONE -- Box.instantiate1 : Expr → Expr → Expr. Actually just instantiate mvars. Except for delay assigned mvars, because with will deal with those using And binders.
 
 
+-/
+
+/-- Replace all occurrences of a variable with `new`. -/
+def instantiateMVarWith (var e new : Expr) : CoreM Expr :=
+  Core.transform e (post := (if · == var then return .done new else return .continue))
 
 
+/--
+Collect the metavariables that appear in an expression.
+This is used after running a tactic, on the metavariable goal.
+-/
+def collectDelayMVarApps (mvarId : MVarId) : MetaM (Std.HashSet MVarId × Std.HashMap MVarId (Array Expr)) := do
+  let e ← instantiateMVars (.mvar mvarId)
+  let (_, res) ← StateT.run (s := ({}, {})) <| Core.transform e (pre := fun e => do
+    if let .mvar mvarId := e then
+      let s : Std.HashSet MVarId × Std.HashMap MVarId (Array Expr) ← get
+      if ← mvarId.isDelayedAssigned then
+        let args := e.getAppArgs
+        if !s.2.contains mvarId then
+          set (s.1, s.2.insert mvarId args)
+      else
+        set (s.1.insert mvarId, s.2)
+    return .continue)
+  return res
+#check collectMVars
+#check Tactic.getU
+#check MetavarContext.collectForwardDeps
+
+#check Core.transform
+
+#check Lean.Expr.instantiate1
 end Box
 
 end HumanProof
+/-
+?a : Nat
+h : ?a = 1
+?b : Nat
+
+⊢
+
+-/
+
+/-
+let ?a := ?b + 1
+-/
+open Lean Meta Elab
+
+elab "test" e:tactic : tactic => do
+  -- let e ← Term.elabTerm e none
+  -- logInfo m! "{e}"
+  let mvarId ← Tactic.getMainGoal
+  Tactic.evalTactic e
+  let mvarIdNew ← Tactic.getMainGoal
+  liftMetaM do
+  logInfo m! "{repr mvarId}; {← instantiateMVars <| Expr.mvar mvarId}"
+  logInfo m! "{repr mvarIdNew}; {← instantiateMVars <| Expr.mvar mvarIdNew}"
+  let (_, mvars) ← collectMVars (.mvar mvarId) |>.run {}
+  for mvar in mvars.result do
+    logInfo m! "{repr mvar}; {← instantiateMVars <| Expr.mvar mvar}; {mvar}"
+    if let some x ← getDelayedMVarAssignment? mvar then
+      logInfo m! "delayed assigment of {Expr.mvar mvar}: {Expr.mvar x.mvarIdPending}"
+set_option pp.instantiateMVars false
+example {P : α → Prop} (x : α) (y : α) {β : Type} (h': True) (h : α = β) (z : Nat) : P x := by
+  -- -- clear y
+  -- rw [h] at y
+  test rw [h] at y
+#check Exists.casesOn
+example {P : α → Prop} (h : ∃ x, P x) (a : Nat) : False := by
+  test cases h
+
+example {α β : Nat} (P : Nat → Prop) (h : P α) (h' : α = β) : False := by
+  test rw [h'] at h
+
+example {α β : Nat} (h' : 15 = β) (h : True) : False := by
+  test induction β generalizing h
+
+example {p q : Prop} (h : p) (g : False) : q := by
+  contrapose h
