lakefile.lean
@@ -6,6 +6,7 @@ package «HumanProof» where
 
 lean_lib «HumanProof» where
   -- add library configuration options here
+  leanOptions := #[⟨`autoImplicit, false⟩]
 
 @[default_target]
 lean_exe «humanproof» where
